\begin{exercises}

	\begin{problist}

	\prob Find the complementary and particular solutions for the following ODEs
	\begin{enumerate}
		\item $y''-2y'-3y=3e^{2t}$
		\item $y''-2y'-3y=-3te^{-t}$
		\item $y''-9y=t^2e^{-3t}-6$
		\item $y''+2y'-8y=e^{-t}-2e^t$
		\item $y''-y'-6y=\sin(t)$
		\item $y''-y'-6y=\sin(t)+3e^{3t}$
		\item $y''+4y=(2t+1)\sin(t) + 4\cos(2t)$
		\item $y''+y=\cos(2t)+t^3$
		\item $y''-y'-2y=t\cos(t) - t\sin(t)$
		\item $y''+5y'+6y = 2e^{-2t}$
	\end{enumerate}



	\prob What is the form of the particular solution for the ODE
	\begin{multline*}
		y^{(6)} + y^{(5)} -5 y^{(4)} + 31 y'''-176y''+220y' \\
			= (3t-1)e^{2t} + t^3e^{-5t}\sin(3t) + (4t^2-2t) e^{-2t} \sin(3t),
	\end{multline*}
	knowing that 
	\begin{multline*}
		x^6 + x^5 - 5 x^4 + 31 x^3 - 176 x^2 + 220 x \\
			= \big((x^2+2)+9\big)*(x-2)^2*x*(x+5)\quad ?
	\end{multline*}

	\prob What is the form of the particular solution for the ODE
	\begin{multline*}
		y'''' - 4 y''' + 10y'' - 12 y' + 5y \\
			= t e^t + t^2 \cos(2t) - (2t+1) e^t \sin(t),
	\end{multline*}
	knowing that 
	\begin{multline*}
		x^4 - 4x^3 + 10 x^2 - 12 x + 5 \\
			= (x-1)^2 \big( (x-1)^2+4\big)\quad  ?
	\end{multline*}

	\prob Consider the ODE
	$$
	t^2 y''+ty'-9y = 0,
	$$
	and a solution $y_1(t) = t^3$.
	
	\begin{enumerate}
		\item Use the reduction of order technique to deduce the general solution to this problem.
		
		\item[\bf Hint.] You should find a second-order ODE for $u(t)$ without the term $u(t)$. So define $v(t) = u'(t)$ and solve the first-order ODE for $v(t)$.
		
		
			%	Solution: $tu'' + 7 u' = 0$ \\
			%	Define: $v = u'$ \\
			%	Solve: $tv' + 7 v = 0 \Rightarrow v = c_2 t^{-7}$ \\
			%	Then: $u = \int v = c_2 \int e^{t^2} dt + c_1$


		
		
		\item Find the solution with initial conditions $y(1)=1$ and $y'(1)=-3$.
		\item Find the solution with initial conditions $y(1)=1$ and $y'(1)=3$.
		\item Find the solution with initial conditions $y(1)=1$ and $y'(1)=0$.
	\end{enumerate}


	\prob Consider the ODE
	$$
	t^2 y'' - 3 t y' + 4 y = 0
	$$
	and a solution $y_1(t) = t^2$.
	
	\begin{enumerate}
		\item Use the reduction of order technique to deduce the general solution to this problem.
		
	
			%	Solution: $tu'' + 7 u' = 0$ \\
			%	Define: $v = u'$ \\
			%	Solve: $tv' + 7 v = 0 \Rightarrow v = c_2 t^{-7}$ \\
			%	Then: $u = \int v = c_2 \int e^{t^2} dt + c_1$
		
		\item Find the solution with initial conditions $y(1)=1$ and $y'(1)=2$.
		\item Find the solution with initial conditions $y(1)=0$ and $y'(1)=1$.
	\end{enumerate}



	
	\prob Consider the ODE $a y'' +by'+cy = f(t)$, with complementary solution $y_c(t) =c_1 y_1(t) + c_2 y_2(t)$ and particular solution $y_p(t)$.
	
	Consider also the initial conditions $y(0)=y_0$ and $y'(0)=v_0$.
	
	Show that there exist constants $c_1, c_2$ such that $y(t) = y_c(t) + y_p(t)$ solves the ODE with these initial conditions.
	
	\end{problist}
\end{exercises}
