\begin{exercises}

	\begin{problist}
	\prob Consider the initial-value problem
	$$ 	\begin{cases}
			 x_{k+1} = 3 x_k + 4 \\
			 x_0 = 1
 		\end{cases} $$
 	\begin{enumerate}
 		\item Using the expand-until-you-find-the-pattern technique, find the solution of this problem.
 		\item Observe that this problem has an equilibrium solution $x^\star$. What is $x^\star$?
 		\item Define a new sequence $y_k = x_k - x^\star$. Which initial-value problem does ti satisfy?
 		\item Find $y_k$.
 		\item Find $x_k$.
 	\end{enumerate}

	\prob Find the solution to the problem
	$$ 	\begin{cases}
			 x_{k+1} = -2x_{k} +3 \\
			 x_1 = 2
 		\end{cases} $$

	\prob When we were solving ODEs, we considered exponential solutions of the form $u_k = e^{rk}$, but above we considered $u_k = r^k$. Are these equivalent?
	
	Consider the initial-value problem
	$$ 	\begin{cases}
			 x_{k+1} = x_{k} - x_{k-1} \\
			 x_0 = 1 \\
			 x_1 = 2
 		\end{cases} $$

	\begin{enumerate}
		\item Solve the problem assuming the solution is of the form $u_k = r^k$.
		\item Solve the problem assuming the solution is of the form $u_k=e^{rk}$.
		\item What can you conclude?
	\end{enumerate}


	\prob Find the solution to the problem
	$$ 	\begin{cases}
			 x_{k+1} = -2x_{k} - x_{k-1} \\
			 x_0 = 1 \\
			 x_1 = 2
 		\end{cases} $$
	
	\prob Find the solution for the problem
	$$ 	\begin{cases}
			 a x_{k+1} - x_k + (1-a) x_{k-1} = 0 \\
			 x_0 = 1 \\
			 x_N = 0
 		\end{cases} $$
	
	
	\prob Consider the problem
	$$ 	x_{k} - 2x_{k-1}  - x_{k-2} + 2 x_{k-3} = 0 $$
	Find the solution for the following initial conditions.
	\begin{enumerate}
		\item $x_0 = 2, x_1 = 2,	 x_2 = 2$.
		\item $x_0 = 1, x_1 = 0,	 x_2 = 1$.
		\item $x_0 = 1, x_1 = 2,	 x_2 = 3$.
	\end{enumerate}
	
	\prob Consider the problem
	$$ 	\begin{cases}
			 x_{k+1} = -2x_{k} - 2x_{k-1} \\
			 x_0 = 1 \\
			 x_1 = 0 
 		\end{cases} $$
 	\begin{enumerate}
 		\item Find the solution of this problem (it will involve complex numbers).
 		\item Show that $x_k \in \mathbb{R}$ for all $k=0,1,\ldots$
	\end{enumerate}
 	Let us re-write the solution without using complex numbers.
 	\begin{enumerate}[resume]
 		\item Assuming the solution is an exponential $x_k=r^k$, what are the possible values or $r$?
	\end{enumerate}
	This means that the solution is of the form
 		$$ x_k = c_1 r_1^k + c_2 r_2^k.$$
 	We need to know how to easily write $\alpha + i \beta)^k$.
 	\begin{enumerate}[resume]
 		\item Using Euler's Formula in \ref{EulersFormula}, write the complex numbers $r_1$ and $r_2$ in the form
			$$ r_1 = \rho e^{i \theta}.$$
			Also show that 
			$$ r_2 = \rho e^{-i \theta}.$$
		\item Now it should be easier to compute $r_1^k$ and $r_2^k$. After simplifying, use Euler's Formula in \ref{EulersFormula} again to get an expression for $r_1^k$ with $\cos$ and $\sin$.
		\item Let us put everything together again to get a solution of the form
		$$ x_k = a_1 \rho^k \cos(?) + a_2 \rho^k \sin(?).$$
		How do $a_1, a_2$ relate to $c_1,c_2$?
		\item Find the constants $a_1,a_2$.
 	\end{enumerate}
	
	
	\end{problist}
\end{exercises}

